theories/dcalc/DCBigStep.v
@@ -1,0 +1,414 @@
+Require Import List.
+Require Import MyTactics.
+Require Import MySequences.
+Require Import DCSyntax.
+Require Import DCFreeVars.
+Require Import DCValues.
+Require Import DCValuesRes.
+Require Import DCReduction.
+
+(* -------------------------------------------------------------------------- *)
+(* -------------------------------------------------------------------------- *)
+
+(* A big-step call-by-value semantics. *)
+
+Inductive bigcbv : term -> term -> Prop :=
+| BigcbvValue:
+  forall v,
+  is_value v ->
+  bigcbv v v
+| BigcbvApp:
+  forall t1 t2 u1 v2 v,
+  bigcbv t1 (Lam u1) ->
+  bigcbv t2 v2 ->
+  ~ is_error v2 ->
+  bigcbv u1.[v2/] v ->
+  bigcbv (App t1 t2) v
+| BigcbvAppConflict1:
+  forall t1 t2,
+  bigcbv t1 Conflict ->
+  bigcbv (App t1 t2) Conflict
+| BigcbvAppConflict2:
+  forall t1 t2 u1,
+  bigcbv t1 (Lam u1) ->
+  bigcbv t2 Conflict ->
+  bigcbv (App t1 t2) Conflict
+| BigcbvAppEmpty1:
+  forall t1 t2,
+  bigcbv t1 Empty ->
+  bigcbv (App t1 t2) Empty
+| BigcbvAppEmpty2:
+  forall t1 t2 u1,
+  bigcbv t1 (Lam u1) ->
+  bigcbv t2 Empty ->
+  bigcbv (App t1 t2) Empty
+| BigcbvDefaultJTrue:
+  forall ts vs tj tc v,
+  List.Forall2 bigcbv ts vs ->
+  List.Forall (eq Empty) vs ->
+  bigcbv tj (Const true) ->
+  bigcbv tc v ->
+  bigcbv (Default ts tj tc) v
+| BigcbvDefaultJFalse:
+  forall ts vs tj tc,
+  List.Forall2 bigcbv ts vs ->
+  List.Forall (eq Empty) vs ->
+  bigcbv tj (Const false) ->
+  bigcbv (Default ts tj tc) Empty
+| BigcbvDefaultV:
+  forall ts vs vs1 v vs2 tj tc,
+  vs = vs1 ++ v :: vs2 ->
+  List.Forall2 bigcbv ts vs ->
+  List.Forall (eq Empty) vs1 ->
+  List.Forall (eq Empty) vs2 ->
+  v <> Empty ->
+  bigcbv (Default ts tj tc) v
+| BigcbvDefaultConflict:
+  forall ts vs vs1 v1 vs2 v2 vs3 tj tc,
+  vs = vs1 ++ v1 :: vs2 ++ v2 :: vs3 ->
+  List.Forall2 bigcbv ts vs ->
+  v1 <> Empty ->
+  v2 <> Empty ->
+  bigcbv (Default ts tj tc) Conflict
+.
+
+Check bigcbv_ind.
+
+Theorem bigcbv_ind'
+: forall P : term -> term -> Prop,
+(forall v : term, is_value v -> P v v) ->
+(forall (t1 t2 : term) (u1 : {bind term}) (v2 v : term),
+ bigcbv t1 (Lam u1) ->
+ P t1 (Lam u1) ->
+ bigcbv t2 v2 ->
+ P t2 v2 ->
+ ~ match v2 with
+   | Empty | Conflict => True
+   | _ => False
+   end -> bigcbv u1.[v2/] v -> P u1.[v2/] v -> P (App t1 t2) v) ->
+(forall t1 t2 : term,
+ bigcbv t1 Conflict -> P t1 Conflict -> P (App t1 t2) Conflict) ->
+(forall (t1 t2 : term) (u1 : {bind term}),
+ bigcbv t1 (Lam u1) ->
+ P t1 (Lam u1) ->
+ bigcbv t2 Conflict -> P t2 Conflict -> P (App t1 t2) Conflict) ->
+(forall t1 t2 : term,
+ bigcbv t1 Empty -> P t1 Empty -> P (App t1 t2) Empty) ->
+(forall (t1 t2 : term) (u1 : {bind term}),
+ bigcbv t1 (Lam u1) ->
+ P t1 (Lam u1) -> bigcbv t2 Empty -> P t2 Empty -> P (App t1 t2) Empty) ->
+(forall (ts vs : list term) (tj tc v : term),
+ Forall2 bigcbv ts vs ->
+ Forall2 P ts vs ->
+ Forall (eq Empty) vs ->
+ bigcbv tj (Const true) ->
+ P tj (Const true) -> bigcbv tc v -> P tc v -> P (Default ts tj tc) v) ->
+(forall (ts vs : list term) (tj tc : term),
+ Forall2 bigcbv ts vs ->
+ Forall2 P ts vs ->
+ Forall (eq Empty) vs ->
+ bigcbv tj (Const false) ->
+ P tj (Const false) -> P (Default ts tj tc) Empty) ->
+(forall (ts vs vs1 : list term) (v : term) 
+   (vs2 : list term) (tj tc : term),
+ vs = vs1 ++ v :: vs2 ->
+ Forall2 bigcbv ts vs ->
+ Forall2 P ts vs ->
+ Forall (eq Empty) vs1 ->
+ Forall (eq Empty) vs2 -> v <> Empty -> P (Default ts tj tc) v) ->
+(forall (ts vs vs1 : list term) (v1 : term) 
+   (vs2 : list term) (v2 : term) (vs3 : list term) 
+   (tj tc : term),
+ vs = vs1 ++ v1 :: vs2 ++ v2 :: vs3 ->
+ Forall2 bigcbv ts vs ->
+ Forall2 P ts vs ->
+ v1 <> Empty -> v2 <> Empty -> P (Default ts tj tc) Conflict) ->
+forall t t0 : term, bigcbv t t0 -> P t t0.
+Admitted.
+
+
+Global Hint Constructors bigcbv : bigcbv.
+
+(* The tactic [invert_bigcbv] looks for a hypothesis of the form [bigcbv t v]
+   and inverts it. *)
+
+Ltac invert_bigcbv :=
+  pick bigcbv invert;
+  try solve [ false; eauto 3 with obvious ].
+
+(* -------------------------------------------------------------------------- *)
+
+(* If [bigcbv t v] holds, then [v] must be a value. *)
+
+Lemma is_value_res_bigcbv:
+  forall t, is_value_res t -> bigcbv t t.
+Proof.
+  intros t Ht.
+  eapply BigcbvValue.
+  induction t; simpl in *; eauto.
+Qed.
+
+Lemma bigcbv_is_value:
+  forall t v,
+  bigcbv t v ->
+  is_value v.
+Proof.
+  induction 1 using bigcbv_ind'; subst; inverts_Forall; simpl; eauto.
+Qed.
+
+Lemma bigcbv_is_value_refl:
+  forall t v,
+  bigcbv t v ->
+  is_value t ->
+  t = v.
+Proof.
+  induction 1 using bigcbv_ind'; intros; simpl in *; tryfalse; eauto.
+Qed.
+
+ 
+
+Global Hint Resolve bigcbv_is_value is_value_res_bigcbv bigcbv_is_value_refl: is_value obvious.
+
+(* -------------------------------------------------------------------------- *)
+
+(* If [t] evaluates to [v] according to the big-step semantics,
+   then [t] reduces to [v] according to the small-step semantics. *)
+
+Lemma bigcbv_star_cbv:
+  forall t v,
+  bigcbv t v ->
+  star cbv t v.
+Proof.
+(* 
+  (* A detailed proof: *)
+  induction 1.
+  (* BigcbvValue *)
+  { eapply star_refl. }
+  (* BigcbvApp *)
+  { eapply star_trans with (App (Lam u1) v2). obvious.
+    eapply star_trans with (App (Lam u1) t2). obvious.
+    eapply star_step. obvious.
+    eauto. }
+  (* BigcbvLet *)
+  { eapply star_trans. obvious.
+    eapply star_step. obvious.
+    eauto. }
+  {
+    eapply star_trans with (Match VariantNone t1 t2).
+    { clear -IHbigcbv1. induction IHbigcbv1.
+      * eapply star_refl.
+      * eapply star_step; obvious.
+    }
+    eapply star_step. obvious.
+    eauto.
+  }
+  {
+    eapply star_trans with (Match (VariantSome vc) t1 t2).
+    { clear -IHbigcbv1. induction IHbigcbv1;
+      eauto with sequences obvious.
+    }
+    eapply star_step. obvious.
+    eauto.
+  }
+  {
+    { clear -IHbigcbv. induction IHbigcbv;
+      eauto with sequences obvious. }
+  } *)
+  (* A much shorter proof: *)
+  induction 1 using bigcbv_ind'; eauto 6 with sequences obvious.
+  * eapply star_trans with (App (Lam u1) t2). {
+      eapply star_cbv_AppL; eauto.
+      eapply star_cbv_is_error; eauto.
+    }
+    eapply star_trans with (App (Lam u1) v2). { obvious. }
+    eapply star_step. { eapply RedBetaV; asimpl; obvious. induction v2; eauto. }
+    eauto.
+  * admit. (* incorrect rules *)
+  * admit. (* incorrect rules *)
+  * admit. (* incorrect rules *)
+  * admit. (* incorrect rules *) 
+  * (* i need some external lemmas here. *) 
+    admit.
+  * admit.
+  * admit.
+  * admit.
+Admitted.
+
+(* Conversely, if [t] reduces to [v] in the small-step semantics,
+   then [t] evaluates to [v] in the big-step semantics. *)
+
+
+Lemma is_value_res_is_value:
+  forall v,
+  is_value_res v -> is_value v.
+Proof.
+  induction v; simpl in *; eauto.
+Qed.
+
+Global Hint Resolve is_value_res_is_value: is_value is_value_res obvious.
+
+Lemma cbv_bigcbv_bigcbv:
+  forall t1 t2,
+  cbv t1 t2 ->
+  forall v,
+  bigcbv t2 v ->
+  bigcbv t1 v.
+Proof.
+  (* A shorter proof: *)
+  induction 1; intros; subst; try solve [ false; tauto
+  | econstructor; eauto with bigcbv
+  | invert_bigcbv; eauto with bigcbv
+  ].
+  * eapply BigcbvApp; eauto using bigcbv.
+    induction v; simpl in *; eauto.
+  * admit.
+  * admit.
+  * inverts_Forall.
+    assert (is_value Conflict). { simpl; eauto. }
+    assert (v = Conflict). { symmetry; eapply bigcbv_is_value_refl; eauto. } subst.
+    eapply BigcbvDefaultConflict.
+    4: exact H2.
+    3: exact H1.
+    1: {
+      assert (Heq: ts1 ++ ti :: ts2 ++ tj :: ts3 = ts1 ++ ti :: ts2 ++ tj :: ts3). { reflexivity. }
+      apply Heq.
+    }
+
+    repeat match goal with
+    | [ |- List.Forall2 _ ( _ ++ _ ) (_ ++ _)] => eapply Forall2_app
+    | [ |- List.Forall2 _ ( _ :: _ ) (_ :: _)] => eapply Forall2_cons
+    end.
+
+    all: try eauto with obvious.
+
+    all: match goal with [ |- List.Forall2 bigcbv ?ts _ ] =>
+    induction ts; econstructor; inverts_Forall; eauto with obvious end.
+  * eapply BigcbvDefaultV.
+    { assert (Heq: ts1 ++ v :: ts2 = ts1 ++ v :: ts2). { reflexivity. }
+      eapply Heq.
+    }
+    {
+      repeat match goal with
+      | [ |- List.Forall2 _ ( _ ++ _ ) (_ ++ _)] => eapply Forall2_app
+      | [ |- List.Forall2 _ ( _ :: _ ) (_ :: _)] => eapply Forall2_cons
+      end.
+
+      all: try eauto with obvious.
+
+      all: match goal with [ |- List.Forall2 bigcbv ?ts _ ] =>
+      induction ts; econstructor; inverts_Forall; eauto with obvious end.
+    }
+    all: eauto.
+
+    assert (Heq: ti = v).
+    { eapply bigcbv_is_value_refl; eauto with obvious. }
+    rewrite <- Heq; eauto.
+  * assert (forall ts ts' vs tj tc v,
+      bigcbv (Default ts tj tc) v ->
+      List.Forall2 bigcbv ts vs ->
+      List.Forall2 bigcbv ts' vs ->
+      bigcbv (Default ts' tj tc) v
+    ).
+    { 
+      inversion 1; intros; simpl in *; tryfalse; subst; admit.
+    }
+    eapply H3.
+    eapply H2.
+    inverts H2; tryfalse.
+    { inverts_Forall.
+      repeat match goal with
+      | [ |- List.Forall2 _ ( _ ++ _ ) _] => eapply Forall2_app
+      | [ |- List.Forall2 _ ( _ :: _ ) _] => eapply Forall2_cons
+      end.
+      - eapply H4.
+      eauto.
+
+    }
+
+Qed.
+
+Lemma star_cbv_bigcbv:
+  forall t v,
+  star cbv t v ->
+  is_value v ->
+  bigcbv t v.
+Proof.
+  induction 1; eauto using cbv_bigcbv_bigcbv with bigcbv.
+Qed.
+
+(* In conclusion, we have the following equivalence: *)
+
+Lemma star_cbv_bigcbv_eq:
+  forall t v,
+  (star cbv t v /\ is_value v) <-> bigcbv t v.
+Proof.
+  split; intros; unpack;
+  eauto using star_cbv_bigcbv, bigcbv_star_cbv with is_value.
+Qed.
+
+(* -------------------------------------------------------------------------- *)
+(* -------------------------------------------------------------------------- *)
+
+(* Suppose the big-step semantics [bigcbv] is taken as the primary definition
+   of the meaning of terms. Then, in terms of [bigcbv], we can define a
+   relation [sim] between terms, which has the flavor of a small-step
+   reduction relation. *)
+
+(* The definition is as follows: if, whenever [u] can produce the value [v],
+   [t] can produce [v] as well, then [t] simulates [u]. *)
+
+Definition sim t u :=
+  forall v,
+  bigcbv u v ->
+  bigcbv t v.
+
+(* This simulation relation is reflexive and transitive, hence a preorder. *)
+
+Lemma reflexive_sim:
+  forall t,
+  sim t t.
+Proof.
+  unfold sim. eauto.
+Qed.
+
+Lemma transitive_sim:
+  forall t1 t2 t3,
+  sim t1 t2 ->
+  sim t2 t3 ->
+  sim t1 t3.
+Proof.
+  unfold sim. eauto.
+Qed.
+
+Global Hint Resolve reflexive_sim transitive_sim : sim.
+
+(* This simulation relation includes the small-step relation [cbv]. *)
+
+Lemma cbv_sim:
+  forall t u,
+  cbv t u ->
+  sim t u.
+Proof.
+  (* This is a direct consequence of the fact that the composition
+     [cbv . bigcbv] is a subset of [bigcbv] -- a fact that was proved above. *)
+  unfold sim. eauto using cbv_bigcbv_bigcbv.
+Qed.
+
+(* As a consequence, [star cbv] is also a subset of [sim]. *)
+
+Lemma star_cbv_sim:
+  forall t u,
+  star cbv t u ->
+  sim t u.
+Proof.
+  induction 1; eauto using cbv_sim with sim.
+Qed.
+
+(* The converse is not true. Clearly, [star cbv] forbids all reductions under
+   a lambda-abstraction, whereas (somewhat nonobviously) [sim] allows certain
+   reductions under lambda-abstractions: intuitively, it allows all necessary
+   reductions, in a certain sense (?). *)
+
+(* For this reason, [sim] can be more comfortable to work with than [star cbv].
+   The proof of correctness of the CPS transformation in CPSCorrectnessBigStep
+   provides an example. *)
